State functional_correctness

EasyCrypt/statement.ec
@@ -1,24 +1,41 @@
+require import AllCore IntDiv CoreMap List Distr.
+
 require import Oram.
 require import SimpleORAM.
+require import SBArray48_32.
+require import SBArray1536_48.
+require import SBArray196608_1536.
 
+from Jasmin require import JModel_x86.
 
 module Jasmin = M(Syscall).
 
+print SBArray48_32.get_sub64.
+
 clone SimpleORAM as EC_Model with
-  type value <- W64.t,
+  type value <- BArray32.t,
   type cell <- W64.t.
 
+type Block = BArray32.t.
 type NodeElem = BArray48.t.
 type Node = BArray1536.t.
 type ORAM = BArray196608.t.
 type PosArray = BArray512.t.
 type PosArray_ORAM = PosArray * ORAM.
 
+op Block_get (vs : Block) (j : int) : W64.t = BArray32.get64 vs j.
+op NodeElem_i (elem : NodeElem) : W64.t = BArray48.get64 elem 0.
+op NodeElem_pos (elem : NodeElem) : W64.t = BArray48.get64 elem 1.
+op NodeElem_vals (elem : NodeElem) : BArray32.t = SBArray48_32.get_sub64 elem 2.
+op NodeElem_get (elem : NodeElem) (j : int) : W64.t = BArray48.get64 elem (2 + j).
+op Node_get (node : Node) (k : int) : NodeElem = SBArray1536_48.get_sub64 node k.
+op ORAM_get (oram : ORAM) (ix : int) : Node = SBArray196608_1536.get_sub64 oram ix.
+op PosArray_get (Pos : PosArray) (i : int) : W64.t = BArray512.get64 Pos i.
+
 op eq_pos_path (pos : W64.t) (p : EC_Model.path) : bool =
   size p <= 64 /\ forall (i : int), 0 <= i < 64 => pos.[i] = nth false p i.
-  
 
-op eq_NodeElem_block (nodeElem : NodeElem) (b : EC_Model.path) : bool. (* TODO *)
+op eq_NodeElem_block (nodeElem : NodeElem) (b : EC_Model.block) : bool. (* TODO *)
 
 op eq_Node_blocklist (node : Node) (b : EC_Model.block list) : bool. (* TODO *)
 
@@ -29,24 +46,24 @@ op eq_Pos_positions (Pos : PosArray) (positions : W64.t -> EC_Model.path) : bool
 op eq_PosORAM_oram (Pos_joram : PosArray_ORAM) (oram : EC_Model.oram) : bool. (* TODO *)
 
 
-type Query = W64.t * W64.t * W64.t.
-type Queries = BArray2400.t.
-type MultiQueryAns = BArray800.t.
+type BlockQuery = W64.t * W64.t * Block.
+type BlockQueries = BArray4800.t.
+type BlockMultiQueryAns = BArray3200.t.
 
-op eq_Query_inst (q : Query) (i : EC_Model.inst) : bool. (* TODO *)
-op eq_Queries_prog (queries : Queries) (p : EC_Model.prog) : bool. (* TODO *)
-op eq_MultiQueryAns_valuelist (ans : MultiQueryAns) (os : W64.t list) : bool. (* TODO *)
+op eq_BlockQuery_inst (q : BlockQuery) (i : EC_Model.inst) : bool. (* TODO *)
+op eq_BlockQueries_prog (queries : BlockQueries) (p : EC_Model.prog) : bool. (* TODO *)
+op eq_BlockMultiQueryAns_valuelist (ans : BlockMultiQueryAns) (os : BArray32.t list) : bool. (* TODO *)
 
 op eq_JLeakage_leakagelist (jleak : JLeakage.leakage) (ecleak : EC_Model.leakage list) : bool. (* TODO *)
 
 
 lemma functional_correctness :
   equiv[
-    Jasmin.multiQuery ~ EC_Model.ORAM.compile :
+    Jasmin.multiQuery_blocks ~ EC_Model.ORAM.compile :
       eq_PosORAM_oram (pos{1}, oram{1}) o{2}
-      /\ eq_Queries_prog queries{1} p{2}
+      /\ eq_BlockQueries_prog queries{1} p{2}
       ==> eq_JLeakage_leakagelist res{1}.`1 EC_Model.ORAM.leakage{2}
-        /\ eq_MultiQueryAns_valuelist res{1}.`4 res{2}.`2
+        /\ eq_BlockMultiQueryAns_valuelist res{1}.`4 res{2}.`2
   ].
 
 
